# Corrigendum


## Section 1.6.3, Page 17, Code 1.2, Line 1 and Line 23

```CloseFormAgent```

#### $\Downarrow$

```ClosedFormAgent```


## Section 2.2.3, Page 43, Example 2.9, First block math

$v_\pi\left(\text{hungry}\right)=-\frac34+\frac45\left(\frac12 v_\pi\left(\text{hungry}\right)+\frac{15}{24}v_\pi\left(\text{full}\right)\right)$

$v_\pi\left(\text{full}\right)=-\frac23+\frac45\left(\frac12v_\pi\left(\text{hungry}\right)+\frac9{24}v_\pi\left(\text{full}\right)\right)$

#### $\Downarrow$

$v_\pi\left(\text{hungry}\right)=-\frac34+\frac45\left(\frac12v_\pi\left(\text{hungry}\right)+\frac12v_\pi\left(\text{full}\right)\right)$

$v_\pi\left(\text{full}\right)=-\frac23+\frac45\left(\frac58v_\pi\left(\text{hungry}\right)+\frac38v_\pi\left(\text{full}\right)\right)$


## Section 2.3, Page 50, Last line

import concept

#### $\Downarrow$

important concept


## Section 2.3.1, Page 51, First block math

$\eta_ \pi\left(\mathsfit{s}\right)\stackrel{\text{def}}=\sum_ {\tau=1}^{+\infty}\gamma^\tau\text{Pr}_ \pi\left[{\mathsfit{S}_ \tau=\mathsfit{s}}\right]$

#### $\Downarrow$

$\eta_ \pi\left(\mathsfit{s}\right)\stackrel{\text{def}}=\sum_ {\tau=0}^{+\infty}\gamma^\tau\text{Pr}_ \pi\left[{\mathsfit{S}_ \tau=\mathsfit{s}}\right]$


## Section 2.3.1, Page 51, Third block math

$\rho_ \pi\left(\mathsfit{s},\mathsfit{a}\right)\stackrel{\text{def}}=\sum_ {\tau=1}^{+\infty}\gamma^\tau\text{Pr}_ \pi\left[{\mathsfit{S}_ \tau=\mathsfit{s},\mathsfit{A}_ \tau=\mathsfit{a}}\right]$

#### $\Downarrow$

$\rho_ \pi\left(\mathsfit{s},\mathsfit{a}\right)\stackrel{\text{def}}=\sum_ {\tau=0}^{+\infty}\gamma^\tau\text{Pr}_ \pi\left[{\mathsfit{S}_ \tau=\mathsfit{s},\mathsfit{A}_ \tau=\mathsfit{a}}\right]$


## Section 2.4.4, Page 67, Second block math, First line

$\frac6{11}$

#### $\Downarrow$

$-10$


## Section 2.4.4, Page 67, Fourth block math

$v_ \ast\left(\text{hungry}\right)=q_ \ast\left(\text{hungry},\text{ignore}\right)=-6,\quad q_ \ast\left(\text{hungry},\text{feed}\right)=-\frac13,$

$v_ \ast\left(\text{full}\right)=q_ \ast\left(\text{full},\text{ignore}\right)=-10,\quad q_ \ast\left(\text{hungry},\text{feed}\right)=5.$

#### $\Downarrow$

$v_ \ast\left(\text{hungry}\right)=q_ \ast\left(\text{hungry},\text{ignore}\right)=-10,\quad q_ \ast\left(\text{hungry},\text{feed}\right)=-\frac13,$

$q_ \ast\left(\text{full},\text{ignore}\right)=-6,\quad v_ \ast\left(\text{full}\right)=q_ \ast\left(\text{hungry},\text{feed}\right)=5.$


## Interdisciplinary Reference 3.1, Page 82, Bullet Group, the Last Bullet Point

$d\left(\mathsfit{x}',\mathsfit{x}'''\right)$

#### $\Downarrow$

$d\left(\mathsfit{x}'',\mathsfit{x}'''\right)$


## Example 4.1, Page 106. 3 occurrences in total, including Fig. 4.1.

$\frac{1-\mathrm{e}^x}{\cos x}$

#### $\Downarrow$

$\frac{1-\mathrm{e}^{-x}}{\cos x}$


## Interdisciplinary Reference 4.2, Page 107, Third Paragraph, the Third Bullet Point

$\sum_{k=0}^{+\infty}{\alpha^2_k}=+\infty$

#### $\Downarrow$

$\sum_{k=0}^{+\infty}{\alpha^2_k}<+\infty$


## Example 4.2, Page 119. 4 occurrences in total.

$\frac{1-\mathrm{e}^x}{\cos x}$

#### $\Downarrow$

$\frac{1-\mathrm{e}^{-x}}{\cos x}$


## Page 154, Second bullet Point of the Bullet Group, First Two Lines. Two occurrence.

$q^{(0)}$

#### $\Downarrow$

$q^{(1)}$


## Page 154, Second bullet Point of the Bullet Group, First Two Lines. Two occurrence.

$q^{(1)}$

#### $\Downarrow$

$q^{(0)}$
